src/lib/sparse/Kuiper.Sparse.Matrix.fst
@@ -207,6 +207,38 @@ instance has_pts_to_smatrix
   pts_to = smatrix_pts_to;
 }
 
+// TODO por que no está definido?
+instance
+is_send_across_pts_to #a r #p n
+: is_send_across (visibility_of r) (Pulse.Lib.Array.PtsTo.pts_to #a r #p n)
+=
+  let i s = is_send_across_pts_to_mask r p s (fun i -> True) in
+  Tactics.Typeclasses.solve
+
+instance is_send_across_smatrix
+  #et {| scalar et |}
+  (#rows #cols : nat)
+  (m : smatrix et rows cols)
+  (vis : visibility)
+  (#_ : squash (visibility_of m.elems == vis))
+  (#_ : squash (visibility_of m.col_ind == vis))
+  (#_ : squash (visibility_of m.row_off == vis))
+  (#f : perm)
+  (v : chest2 et rows cols)
+  : is_send_across vis (smatrix_pts_to m #f v)
+=
+  let open Pulse.Lib.Array.PtsTo in
+  let i_elems elems :
+    is_send_across vis (pts_to m.elems #f elems) =
+    is_send_across_pts_to m.elems #f elems  in
+  let i_col_ind col_ind :
+    is_send_across vis (pts_to m.col_ind #f col_ind) =
+    is_send_across_pts_to m.col_ind #f col_ind  in
+  let i_row_off row_off :
+    is_send_across vis (pts_to m.row_off #f row_off) =
+    is_send_across_pts_to m.row_off #f row_off  in
+  solve
+
 ghost
 fn smatrix_share_n'
   (#et:Type0) {| d : scalar et |}
@@ -379,8 +411,81 @@ fn smatrix_gather_n
   fold smatrix_pts_to m #f em;
 }
 
+let rec mem_slice_lemma
+  (#et : eqtype)
+  (x : et) (s : seq et)
+  (a b : nat {a <= b /\ b <= len s})
+  : Lemma
+    (ensures mem_slice x s a b <==> Seq.mem x (Seq.slice s a b))
+    (decreases (b - a))
+    [SMTPatOr
+      [[SMTPat (mem_slice x s a b)];
+       [SMTPat (Seq.mem x (Seq.slice s a b))]]]
+=
+  if a < b && s @! a <> x
+    then mem_slice_lemma x s (a + 1) b
+    else ()
 
-open Kuiper.Sparse.Array
+let rec index_mem_slice_lemma
+  (#et : eqtype)
+  (x : et) (s : seq et)
+  (a b : nat {a <= b /\ b <= len s})
+  : Lemma
+    (requires mem_slice x s a b /\ Seq.mem x (Seq.slice s a b))
+    (ensures
+      s @! index_mem_slice x s a b ==
+      Seq.slice s a b @! Seq.index_mem x (Seq.slice s a b)
+    )
+    (decreases (b - a))
+=
+  if a < b && s @! a <> x
+    then index_mem_slice_lemma x s (a + 1) b
+    else ()
+
+
+let unsparse_row_lemma
+  (#et:Type0) {| scalar et |}
+  (#nnz rows cols : nat)
+  (elems : lseq et nnz)
+  (col_ind : lseq nat nnz)
+  (row_off : lseq nat (rows + 1))
+  (i : natlt rows)
+  : Lemma
+    (requires valid_smatrix rows cols col_ind row_off)
+    (ensures
+      ematrix_row (smatrix_unsparse rows cols elems col_ind row_off) i ==
+      unsparse
+        ((row_off @! i + 1) - (row_off @! i)) cols
+        (Seq.slice elems (row_off @! i) (row_off @! i + 1))
+        (Seq.slice col_ind (row_off @! i) (row_off @! i + 1))
+    )
+=
+  let m = smatrix_unsparse rows cols elems col_ind row_off in
+  let row = ematrix_row m i in
+
+  let ri = row_off @! i in
+  let re = row_off @! (i + 1) in
+
+  let selems = Seq.slice elems ri re in
+  let spos = Seq.slice col_ind ri re in
+  let s = unsparse (re - ri) cols selems spos in
+
+  introduce forall (j : natlt cols).
+    row @! j == s @! j
+  with (
+    if mem_slice j col_ind ri re
+      then (
+        mem_slice_lemma j col_ind ri re;
+        index_mem_slice_lemma j col_ind ri re;
+        ()
+      )
+      else ()
+  );
+  assert row `Seq.equal` s
+
+(*
+ * Extraer un arreglo sparse de una matriz sparse. No se usa
+
 open Pulse.Lib.Trade
 open Kuiper.Seq.Common
 
@@ -455,80 +560,6 @@ fn gpu_array_paste'
 {
   admit()
 }
-
-let rec mem_slice_lemma
-  (#et : eqtype)
-  (x : et) (s : seq et)
-  (a b : nat {a <= b /\ b <= len s})
-  : Lemma
-    (ensures mem_slice x s a b <==> Seq.mem x (Seq.slice s a b))
-    (decreases (b - a))
-    [SMTPatOr
-      [[SMTPat (mem_slice x s a b)];
-       [SMTPat (Seq.mem x (Seq.slice s a b))]]]
-=
-  if a < b && s @! a <> x
-    then mem_slice_lemma x s (a + 1) b
-    else ()
-
-let rec index_mem_slice_lemma
-  (#et : eqtype)
-  (x : et) (s : seq et)
-  (a b : nat {a <= b /\ b <= len s})
-  : Lemma
-    (requires mem_slice x s a b /\ Seq.mem x (Seq.slice s a b))
-    (ensures
-      s @! index_mem_slice x s a b ==
-      Seq.slice s a b @! Seq.index_mem x (Seq.slice s a b)
-    )
-    (decreases (b - a))
-=
-  if a < b && s @! a <> x
-    then index_mem_slice_lemma x s (a + 1) b
-    else ()
-
-
-#push-options "--z3rlimit 40"
-let unsparse_row_lemma
-  (#et:Type0) {| scalar et |}
-  (#nnz rows cols : nat)
-  (elems : lseq et nnz)
-  (col_ind : lseq nat nnz)
-  (row_off : lseq nat (rows + 1))
-  (i : natlt rows)
-  : Lemma
-    (requires valid_smatrix rows cols col_ind row_off)
-    (ensures
-      ematrix_row (smatrix_unsparse rows cols elems col_ind row_off) i ==
-      unsparse
-        ((row_off @! i + 1) - (row_off @! i)) cols
-        (Seq.slice elems (row_off @! i) (row_off @! i + 1))
-        (Seq.slice col_ind (row_off @! i) (row_off @! i + 1))
-    )
-=
-  let m = smatrix_unsparse rows cols elems col_ind row_off in
-  let row = ematrix_row m i in
-
-  let ri = row_off @! i in
-  let re = row_off @! (i + 1) in
-
-  let selems = Seq.slice elems ri re in
-  let spos = Seq.slice col_ind ri re in
-  let s = unsparse (re - ri) cols selems spos in
-
-  introduce forall (j : natlt cols).
-    row @! j == s @! j
-  with (
-    if mem_slice j col_ind ri re
-      then (
-        mem_slice_lemma j col_ind ri re;
-        index_mem_slice_lemma j col_ind ri re;
-        ()
-      )
-      else ()
-  );
-  assert row `Seq.equal` s
-#pop-options
 
 // TODO: is this useful?
 #push-options "--z3rlimit 40"
@@ -751,3 +782,4 @@ fn smatrix_extract
 
   srow;
 }
+*)
